cleaned up, now with Makefile!

lang.hs
@@ -1,4 +1,0 @@
-
-open_at_end :: [a] -> ([a] -> [a])
-open_at_end [] = id
-open_at_end (x:xs) = \
