Lang.v
@@ -1,53 +1,22 @@
 Require Export SfLib.
 Require Export Permutation.
+Require Import List.
 
-Require Import Misc. 
+Inductive store : Type := 
+  | Empty : store
+  | Extend : store -> id -> nat -> store.
 
-Definition store := partial_map nat.
+Fixpoint gets (i : id) (s : store) : option nat :=
+  match s with 
+    | Empty => None
+    | Extend s' i' n => 
+      if beq_id i i' then 
+        Some n else 
+        gets i s'
+  end.
 
 Inductive uid : Type := 
   | UID : nat -> uid.
-
-Definition beq_uid uid1 uid2 :=
-  match (uid1, uid2) with
-    (UID n1, UID n2) => beq_nat n1 n2
-  end.
-
-Theorem beq_uid_refl : forall i,
-  true = beq_uid i i.
-Proof.
-  intros. destruct i.
-  apply beq_nat_refl.  Qed.
-
-Theorem beq_uid_eq : forall i1 i2,
-  true = beq_uid i1 i2 -> i1 = i2.
-Proof.
-  intros i1 i2 H.
-  destruct i1. destruct i2.
-  apply beq_nat_eq in H. subst.
-  reflexivity.  Qed.
-
-Theorem beq_uid_false_not_eq : forall i1 i2,
-  beq_uid i1 i2 = false -> i1 <> i2.
-Proof.
-  intros i1 i2 H.
-  destruct i1. destruct i2.
-  apply beq_nat_false in H.
-  intros C. apply H. inversion C. reflexivity.  Qed.
-
-Theorem not_eq_beq_uid_false : forall i1 i2,
-  i1 <> i2 -> beq_uid i1 i2 = false.
-Proof.
-  intros i1 i2 H.
-  destruct i1. destruct i2.
-  assert (n <> n0).
-    intros C. subst. apply H. reflexivity.
-  apply not_eq_beq_false. assumption.  Qed.
-
-Theorem beq_uid_sym: forall i1 i2,
-  beq_uid i1 i2 = beq_uid i2 i1.
-Proof.
-  intros i1 i2. destruct i1. destruct i2. apply beq_nat_sym. Qed.
 
 Definition neighbors : Type := (list uid)%type.
 
@@ -61,6 +30,7 @@ Inductive aexp : Type :=
   | APlus : aexp -> aexp -> aexp
   | AMinus : aexp -> aexp -> aexp
   | AMult : aexp -> aexp -> aexp.
+Hint Constructors aexp.
 
 Tactic Notation "aexp_cases" tactic(first) ident(c) :=
   first;
@@ -70,13 +40,14 @@ Tactic Notation "aexp_cases" tactic(first) ident(c) :=
 
 Inductive avalue : aexp -> Prop :=
   | AV_num : forall n, avalue (ANum n).
+Hint Constructors avalue.
 
 Reserved Notation " a '/' st '#' u '==>a' a' " (at level 40, st at level 39, u at level 41).
 Inductive astep : aexp -> store -> uid -> aexp -> Prop :=
   | AS_UId : forall st n, 
                AUId / st # (UID n) ==>a (ANum n)
-   | AS_Id : forall (id : id) (st : store) (u : uid) (n : nat),
-              st id = Some n -> 
+  | AS_Id : forall (id : id) (st : store) (u : uid) (n : nat),
+              gets id st = Some n -> 
               (AId id) / st # u ==>a (ANum n)
   | AS_Plus1 : forall (al al' ar : aexp) (st : store) (u : uid),
                  al / st # u ==>a al' -> 
@@ -106,6 +77,7 @@ Inductive astep : aexp -> store -> uid -> aexp -> Prop :=
   | AS_Minus : forall (nl nr : nat) (st :store) (u : uid),
                 (AMinus (ANum nl) (ANum nr)) / st # u ==>a (ANum (nl - nr))
   where " a '/' st '#' u '==>a' a' " := (astep a st u a').
+Hint Constructors astep.
 
 Inductive aeval : aexp -> store -> uid -> aexp -> Prop :=
   | AE_Value : forall a s u,
@@ -114,6 +86,7 @@ Inductive aeval : aexp -> store -> uid -> aexp -> Prop :=
                 a / s # u ==>a a' -> 
                 aeval a' s u a'' -> 
                 aeval a s u a''.
+Hint Constructors aeval.
 (* Notation " a '/' st '#' u '~~>a' a' " := (aeval a st u a') (at level 39, st at level 38, u at level 40). *)
 
 Inductive bexp : Type := 
@@ -123,6 +96,7 @@ Inductive bexp : Type :=
   | BLe : aexp -> aexp -> bexp
   | BNot : bexp -> bexp
   | BAnd : bexp -> bexp -> bexp.
+Hint Constructors bexp.
 
 Tactic Notation "bexp_cases" tactic(first) ident(c) :=
   first;
@@ -145,6 +119,7 @@ Notation "'B&&'" :=
 Inductive bvalue : bexp -> Prop :=
   | BV_true : bvalue BTrue
   | BV_false : bvalue BFalse.
+Hint Constructors bvalue.
 
 Reserved Notation " b '/' st '#' u '==>b' b' " (at level 40, st at level 39, u at level 41).
 Inductive bstep : bexp -> store -> uid -> bexp -> Prop :=
@@ -195,6 +170,7 @@ Inductive bstep : bexp -> store -> uid -> bexp -> Prop :=
   | BS_AndFalseR : forall (st : store) (u : uid),
                      BAnd BTrue BFalse / st # u ==>b BFalse
   where " b '/' st '#' u '==>b' b' " := (bstep b st u b').
+Hint Constructors bstep.
 
 Inductive beval : bexp -> store -> uid -> bexp -> Prop :=
   | BE_Value : forall a s u,
@@ -203,6 +179,7 @@ Inductive beval : bexp -> store -> uid -> bexp -> Prop :=
                 b / s # u ==>b b' -> 
                 beval b' s u b'' -> 
                 beval b s u b''.
+Hint Constructors beval.
 (* Notation " b '/' st '#' u '~~>b' b' " := (beval b st u b') (at level 50, st at level 49, u at level 51). *)
 
 Inductive com : Type :=
@@ -213,6 +190,7 @@ Inductive com : Type :=
   | CWhile : bexp -> com -> com
   | CSend : neighbor -> aexp -> com
   | CReceive : id -> com.
+Hint Constructors com.
 
 Notation "'DONE'" := 
   CDone.
@@ -241,15 +219,33 @@ Tactic Notation "com_cases" tactic(first) ident(c) :=
 
 Inductive cvalue : com -> Prop :=
   | CV_done : cvalue CDone. 
+Hint Constructors cvalue.
 
 Definition queue : Type := (list nat)%type.
 Definition state : Type := (store * queue)%type.
-Definition empty_state : state := (empty,[]).
+Definition empty_state : state := (Empty,[]).
+
+Fixpoint index {A : Type} (n : nat) (ls : list A) : option A :=
+  match ls with
+  | nil => None
+  | h :: t => 
+    match n with 
+    | O => Some h
+    | S n' => index n' t
+    end
+  end.
+
+Fixpoint pull {A : Type} (q : list A) : option A :=   
+  match q with
+  | nil => None
+  | h :: nil => Some h
+  | (h :: t) => pull t
+  end.
 
 Reserved Notation " c '/' state '#' u '==>c' c' '&' state' " (at level 40, state at level 39, u at level 41).
 Inductive cstep : com -> state -> uid -> com -> state -> Prop :=
-  | CS_AssignVal : forall (id : id) (c : com) (n : nat) (st : store) (q : queue) (u : uid),
-                     (CAssign id (ANum n)) / (st,q) # u ==>c CDone & (extend st id n,q)
+  | CS_AssignVal : forall (id : id) (n : nat) (st : store) (q : queue) (u : uid),
+                     (CAssign id (ANum n)) / (st,q) # u ==>c CDone & (Extend st id n,q)
   | CS_AssignStep : forall (id : id) (a a' : aexp) (st : store) (q : queue) (u : uid), 
                       aeval a st u a' -> 
                       (CAssign id a) / (st,q) # u ==>c (CAssign id a') & (st,q)
@@ -271,12 +267,13 @@ Inductive cstep : com -> state -> uid -> com -> state -> Prop :=
                   (CWhile b c) / (st,q) # u ==>c (CIf b (CSeq c (CWhile b c)) CDone) & (st,q)
   | CS_ReceiveStep : forall (id : id) (n : nat) (rest : list nat) (u : uid) (st : store) (q : queue),
                        pull q = Some n -> 
-                       remove_last q = rest -> 
-                       (CReceive id) / (st,q) # u ==>c CDone & (extend st id n, rest)
+                       removelast q = rest -> 
+                       (CReceive id) / (st,q) # u ==>c CDone & (Extend st id n, rest)
   | CS_SendStep : forall (msg msg' : aexp) (st : store) (q : queue) (u : uid) (nbor : neighbor),
                     aeval msg st u msg' ->
                     (CSend nbor msg) / (st,q) # u ==>c (CSend nbor msg') & (st,q)
   where " c '/' st '#' u '==>c' c' '&' st' " := (cstep c st u c' st').
+Hint Constructors cstep.
 
 Inductive process : Type :=
   | Process : com -> state -> uid -> neighbors -> process.
@@ -287,6 +284,7 @@ Inductive local_step : process -> process -> Prop :=
            c / (st,q) # u ==>c c' & (st',q') -> 
            (Process c (st,q) u n) =local=> (Process c' (st',q') u n)
   where " p '=local=>' p' " := (local_step p p').                                           
+Hint Constructors local_step.
 
 Fixpoint clear_send (p : process) : process :=
   match p with 
@@ -294,11 +292,6 @@ Fixpoint clear_send (p : process) : process :=
   | Process (CSeq (CSend _ _) c') s u n => Process c' s u n
   | _ => p
   end.
-
-Inductive proc_terminates : process -> Prop :=
-  | P_Termination : forall p s u n, 
-                      p =local=> (Process DONE s u n) -> 
-                      proc_terminates p.
 
 Inductive sending_msg_to : process -> nat -> uid -> Prop :=
   | SendingLast : forall s n_ix nbors msg_val u u',
@@ -309,16 +302,18 @@ Inductive sending_msg_to : process -> nat -> uid -> Prop :=
                    index n_ix nbors = Some u' -> 
                    sending_msg_to (Process (CSeq (CSend (Neighbor n_ix) (ANum msg_val)) c') s u nbors)
                                   msg_val u'.
+Hint Constructors sending_msg_to.
 
 Inductive send_step : (process * process) -> (process * process) -> Prop :=
   | SS : forall c c' s st' q' u u' n n' msg,
            sending_msg_to (Process c s u n) msg u' ->
            send_step (Process c s u n, Process c' (st',q') u' n')
                      (clear_send (Process c s u n), Process c' (st',q' ++ [msg]) u' n').
+Hint Constructors send_step.
 
 Inductive system : Type := 
   | System : list process -> system. 
-
+Hint Constructors system.
 
 Inductive step : system -> system -> Prop :=
   | Step_Permute : forall proc_list proc_list',
@@ -335,140 +330,12 @@ Inductive step : system -> system -> Prop :=
                       send_step (sender, receiver) (sender', receiver') ->
                       step (System proc_list)
                            (System (sender' :: (receiver' :: rest))).                            
+Hint Constructors step.
 
 Definition multistep : system -> system -> Prop := multi step.
+Hint Unfold multistep.
+Hint Constructors multi.
+
 Notation "s '!!' s'" :=
   (multistep s s') (at level 30).
-
-Inductive system_halted : system -> Prop :=
-  | SystemHalted : forall p s u n proc_list, 
-                     In p proc_list -> 
-                     p = Process DONE s u n -> 
-                     system_halted (System proc_list).
-
-Inductive system_halts : system -> Prop :=
-  | SystemHalts : forall s s', 
-                    s !! s' -> 
-                    system_halted s' ->
-                    system_halts s. 
-
-Definition leader : id := Id 0.
-Definition finished : id := Id 1.
-Definition msg : id := Id 2.
-Definition leaderA : aexp := (AId leader).
-Definition finishedA : aexp := (AId finished).
-Definition msgA : aexp := (AId msg).
-
-Definition leader_election : com :=
-  leader ::= (ANum 0);
-  finished ::= (ANum 0);
-  SEND AUId TO (Neighbor 0);
-  WHILEB (B= finishedA (ANum 0)) DO
-    msg <-RECEIVE;     
-    IFB (B= msgA (ANum 0))
-    THEN finished ::= (ANum 1)
-    ELSE 
-      IFB (B= msgA AUId)
-      THEN leader ::= msgA;
-           finished ::= (ANum 1);
-           SEND (ANum 0) TO (Neighbor 0)
-      ELSE 
-        IFB (B< AUId msgA)
-        THEN leader ::= msgA;
-             SEND msgA TO (Neighbor 0)
-        ELSE SEND AUId TO (Neighbor 0) 
-        FI
-      FI
-    FI
-  END.
-        
-Definition SystemP2 : system :=
-  System ((Process leader_election empty_state (UID 1) [UID 2]) :: 
-         [Process leader_election empty_state (UID 2) [UID 1]]).
-
-Ltac pull_to_front :=
-  eapply multi_step; [eapply Step_Permute; apply Permutation_cons_append | ].
-
-Tactic Notation "takes_local_step" int_or_var(n) "then" tactic(ts) :=
-  eapply multi_step; 
-  [eapply Step_LocalStep; [ apply Permutation_refl | apply LS; do n (apply CS_SeqStep); ts ] | ].
-Tactic Notation "takes_local_step" "then" tactic(ts) :=
-  takes_local_step 1 then ts.
-Tactic Notation "takes_local_step" int_or_var(n) := 
-  takes_local_step n then idtac.
-Tactic Notation "takes_local_step" := takes_local_step 1.
-Tactic Notation "seq_next" := takes_local_step 0 then (apply CS_SeqNext).
-Tactic Notation "takes_assign_step" := 
-  takes_local_step then (apply CS_AssignVal; apply CDone).
-Tactic Notation "takes_receive_step" :=
-  takes_local_step 2 then 
-    (apply CS_ReceiveStep; reflexivity; apply CDone);
-  takes_local_step 1 then (apply CS_SeqNext).
-Tactic Notation "takes_send_local_step" tactic(ts) := 
-  takes_local_step 1 then (apply CS_SendStep; ts).  
-Tactic Notation "takes_send_step" :=
-  eapply multi_step; 
-  [eapply Step_SendStep; [ apply Permutation_refl
-                         | eapply SS; eapply SendingSeq; reflexivity ] | ].
-Tactic Notation "takes_while_unfold_step" :=
-  takes_local_step 0 then (apply CS_WhileUnfold).
-Tactic Notation "takes_if_step" tactic(ts) := takes_local_step 0 then (apply CS_IfStep; ts).
-Tactic Notation "takes_if_true_step" :=
-  takes_local_step 0 then (apply CS_IfTrue).
-Tactic Notation "takes_if_false_step" := 
-  takes_local_step 0 then (apply CS_IfFalse).
-
-Lemma SystemP2Halts : system_halts SystemP2.
-Proof with simpl. 
-  unfold SystemP2. eapply SystemHalts. unfold leader_election.  
-  do 2 (takes_assign_step; seq_next);
-  takes_local_step then (apply CS_SendStep;
-    eapply AE_Step; [apply AS_UId | apply AE_Value; apply AV_num ]).
-  takes_send_step.
-  takes_while_unfold_step.
-  takes_local_step 0 then (apply CS_IfStep;                           
-    eapply BE_Step; [apply BS_Eq1; 
-                      eapply AE_Step; [apply AS_Id; reflexivity
-                                      | apply AE_Value; apply AV_num ]
-                    | eapply BE_Step; [ apply BS_EqTrue; reflexivity
-                                     | apply BE_Value; apply BV_true ] ]).
-  takes_local_step 0 then (apply CS_IfStep).
-    eapply BE_Step. apply BS_Eq1. eapply AE_Step. apply AS_Id. reflexivity.                          apply AE_Value. apply AV_num. eapply BE_Step. apply BS_EqTrue. reflexivity.
-    apply BE_Value. apply BV_true.
-  takes_if_true_step.
-  pull_to_front.
-  steps_to_receive. simpl.
-  pull_to_front.
-  steps_to_receive. simpl.
-  takes_receive_step.
-  pull_to_front.
-  takes_receive_step.
-  takes_if_step_w_ 1.
-    
-(* Informally, the code I want to execute is the following 
-leader := 0;
-finished := 0
-while not (finished == 0):
-  msg <-RECEIVE
-  if msg == 0:
-    DONE
-  else:
-    if(msg == u) { 
-      leader := u;
-    }
-*)    
-Ltac steps_to_receive := 
-  do 2 (takes_assign_step; seq_next);
-  takes_local_step then (apply CS_SendStep;
-    eapply AE_Step; [apply AS_UId | apply AE_Value; apply AV_num ]);
-  takes_send_step;
-  takes_while_unfold_step;
-  takes_local_step 0 then (apply CS_IfStep;                           
-    eapply BE_Step; [apply BS_Eq1; 
-                      eapply AE_Step; [apply AS_Id; reflexivity
-                                      | apply AE_Value; apply AV_num ]
-                    | eapply BE_Step; [ apply BS_EqTrue; reflexivity
-                                     | apply BE_Value; apply BV_true ] ]);
-  takes_if_true_step.
-
 
