Cases.v
@@ -1,0 +1,311 @@
+Require Import Misc.
+Require Import Lang.
+Require Import Leader. 
+Require Import Coq.Logic.Decidable.
+Require Import ListExt.
+Require Export SfLib.
+
+
+Inductive is_done : process -> Prop :=
+  | cDone : forall s u n, is_done (Process CDone s u n).
+Hint Constructors is_done.
+
+Lemma decidable_is_done : forall p, decidable (is_done p).
+Proof.
+  intros. unfold decidable. destruct p.
+  com_cases (destruct c) Case; 
+    try solve [right; unfold not; intros; inversion H].
+  Case "DONE". 
+    left. constructor.
+Qed.
+
+Inductive is_sending : process -> Prop :=
+  | cSend : forall s u n nbor m, is_sending (Process (CSend (Neighbor nbor) (ANum m)) s u n).
+Hint Constructors is_sending.
+
+Lemma decidable_is_sending : forall p, decidable (is_sending p).
+Proof. 
+  intros. unfold decidable. destruct p.
+  com_cases (destruct c) Case;
+    try solve [right; unfold not; intros; inversion H].
+  Case "SEND";
+    aexp_cases (destruct a) SCase;
+    try solve [right; unfold not; intros; inversion H].
+    SCase "ANum".
+      left. destruct n0.
+      constructor.
+Qed.
+
+Fixpoint isReceiving (c : com) : bool :=
+  match c with 
+    | CSeq c' _ => isReceiving c'
+    | CReceive _ => true
+    | _ => false
+  end.
+
+Inductive is_receiving : process -> Prop :=
+| cReceive : forall c st m msgs u n, 
+               isReceiving c = true -> 
+               is_receiving (Process c (st, m :: msgs) u n).
+Hint Constructors is_receiving.
+
+Lemma decidable_is_receiving : forall p, decidable (is_receiving p).
+Proof.
+  intros. unfold decidable. destruct p.
+  com_cases (induction c) Case;
+    try solve [right; unfold not; intros; inversion H; inversion H1].
+  Case ";".
+    inversion IHc1. 
+    SCase "is_receiving c1". 
+      inversion H. left. constructor. simpl. assumption.
+    SCase "not (is_receiving c1)". 
+      right. unfold not. intro. inversion H0. 
+      assert (is_receiving (Process c1 s u n)).
+      subst. apply cReceive. simpl in H2. assumption. 
+      apply H in H6. assumption.
+  Case "RECEIVE".
+     destruct s. destruct q. 
+     SCase "[]". 
+       right. unfold not; intros. inversion H.
+     SCase "msg :: msgs".
+       left. constructor. reflexivity.
+Qed.
+
+Definition decidable_list_forall {A : Type} (aProp : A -> Prop) := 
+  forall ls,
+    decidable (forall x, In x ls -> aProp x).
+
+(*
+Tactic Notation "decided" constr(prop) "by" constr(lemma) :=
+  assert (decidable prop); apply lemma. 
+*)
+  
+Lemma decidable_in : 
+  forall {A : Type} (a : A) (ls : list A), 
+    (forall (x y : A), decidable (x = y)) -> 
+    decidable (In a ls).
+Proof.
+  intros. unfold decidable. 
+  induction ls as [| l ls']. 
+  Case "[]".
+    right. intro. inversion H0.
+  Case "l :: ls'".
+    inversion IHls'.
+    SCase "In a ls'".
+      left. apply in_cons. assumption.
+    SCase "~ In a ls'".
+      assert (decidable (a = l)).
+      apply H. unfold decidable in H1. inversion H1.
+      SSCase "a = l".
+        left. unfold In. left. rewrite H2. reflexivity. 
+      SSCase "a <> l".
+      right. unfold not. intros. 
+        inversion H3. apply H2. rewrite H4. reflexivity.
+        apply H0 in H4. assumption.
+Qed.      
+
+Lemma decidable_list_forall_if_decidable :
+  forall {A : Type} (P : A -> Prop),
+    (forall (x y : A), decidable (x = y)) -> 
+    (forall (a : A), decidable (P a)) -> 
+    decidable_list_forall P.
+Proof. 
+  unfold decidable_list_forall. intros. unfold decidable. 
+  induction ls as [| x ls']. 
+  Case "[]". left. intros. 
+    inversion H1.
+  Case "x :: ls". 
+    inversion IHls'.
+    SCase "forall".
+      unfold decidable in H0. 
+      assert (decidable (P x)).
+      apply H0. unfold decidable in H2.
+      inversion H2.
+      SSCase "P x".
+        left. intros.
+        inversion H4. rewrite <- H5. assumption.
+        apply H1. assumption.
+      SSCase "~ P x".
+        right. unfold not. intros. unfold not in H3. apply H3.
+        apply H4. apply in_eq.
+   SCase "~ forall".
+     right. unfold not. intros.
+     unfold not in H1.
+     apply H1. intros.
+     apply H2. apply in_cons. assumption.
+Qed.     
+
+Definition decidable_eq (A : Type) : Prop := forall (x y : A), decidable (x = y).
+Hint Unfold decidable_eq.
+
+Tactic Notation "start_dec_eq" ident(x) ident(y) := unfold decidable_eq; induction x; induction y.
+Tactic Notation "dec" constr(a) constr(b) "via" reference(lemma) := assert (a = b \/ a <> b); apply lemma. 
+
+Lemma decidable_id : decidable_eq id.
+Proof. 
+  start_dec_eq x y. assert (n = n0 \/ n <> n0). apply dec_eq_nat. 
+  inversion H. 
+    subst. left. reflexivity.
+    right. unfold not. intro.
+    apply H0. inversion H1. reflexivity.
+Qed. 
+
+Lemma decidable_neighbor : decidable_eq neighbor.
+Proof. 
+  start_dec_eq x y. unfold decidable. decide equality. apply dec_eq_nat.
+Qed. 
+
+Lemma decidable_aexp : decidable_eq aexp.
+Proof. 
+  start_dec_eq x y;
+    try solve [left; reflexivity | right; unfold not; intros; inversion H].
+    assert (decidable (i = i0)).
+      apply decidable_id. inversion H. 
+      left. subst. reflexivity.
+      right. unfold not. unfold not in H0. intros. apply H0. inversion H1. reflexivity.
+    assert (decidable (n = n0)). apply dec_eq_nat.
+    inversion H. 
+      left. subst. reflexivity.     
+      right. unfold not. unfold not in H0. intros. apply H0. inversion H1. reflexivity.
+    assert (decidable (x1 = y1)). apply IHx1.
+    inversion H.
+      assert (decidable (x2 = y2)). apply IHx2. 
+      inversion H1. 
+        subst. left. reflexivity.
+        right. unfold not. intros. 
+        unfold not in H2. apply H2. inversion H3. reflexivity.
+      right. unfold not. intros. unfold not in H0. apply H0. inversion H1. reflexivity.
+    assert (decidable (x1 = y1)). apply IHx1.
+    inversion H.
+      assert (decidable (x2 = y2)). apply IHx2. 
+      inversion H1. 
+        subst. left. reflexivity.
+        right. unfold not. intros. 
+        unfold not in H2. apply H2. inversion H3. reflexivity.
+      right. unfold not. intros. unfold not in H0. apply H0. inversion H1. reflexivity.
+    assert (decidable (x1 = y1)). apply IHx1.
+    inversion H.
+      assert (decidable (x2 = y2)). apply IHx2. 
+      inversion H1. 
+        subst. left. reflexivity.
+        right. unfold not. intros. 
+        unfold not in H2. apply H2. inversion H3. reflexivity.
+      right. unfold not. intros. unfold not in H0. apply H0. inversion H1. reflexivity.
+Qed.        
+
+Tactic Notation "disimilar" :=
+    try solve [left; reflexivity | right; unfold not; intros; inversion H].
+
+Lemma decidable_bexp : decidable_eq bexp.
+Proof. 
+  unfold decidable_eq. intros x y. 
+  generalize dependent y. bexp_cases (induction x) Case; intro y.
+  bexp_cases (induction y) SCase;
+    disimilar. 
+  bexp_cases (induction y) SCase; 
+    disimilar.
+  bexp_cases (induction y) SCase;
+    disimilar.
+  Case "BEq". SCase "BEq".
+  assert (decidable (a = a1)). apply decidable_aexp.
+  inversion H.
+    assert (decidable (a0 = a2)). apply decidable_aexp.
+      inversion H1. 
+        subst. left. reflexivity.
+        right. unfold not. intros. 
+        unfold not in H2. apply H2. inversion H3. reflexivity.
+      right. unfold not. intros. unfold not in H0. apply H0. inversion H1. reflexivity.
+  bexp_cases (induction y) SCase;
+    disimilar.
+  Case "BLe". SCase "BLe".      
+  assert (decidable (a = a1)). apply decidable_aexp.
+  inversion H.
+    assert (decidable (a0 = a2)). apply decidable_aexp.
+      inversion H1. 
+        subst. left. reflexivity.
+        right. unfold not. intros. 
+        unfold not in H2. apply H2. inversion H3. reflexivity.
+      right. unfold not. intros. unfold not in H0. apply H0. inversion H1. reflexivity.
+  Case "BNot". destruct y; try disimilar.
+  assert (decidable (x = y)) by apply IHx.
+  inversion H. subst; left; auto.
+  right. intro C; inversion C; contradiction.
+  Case "BAnd". destruct y; try disimilar. 
+  assert (decidable (x1 = y1)) by apply IHx1.
+  assert (decidable (x2 = y2)) by apply IHx2.
+  inversion H; inversion H0.
+  subst. left. reflexivity.
+  right. unfold not. intro. inversion H3. contradiction.
+  right. unfold not. intro. inversion H3. contradiction.
+  right. unfold not. intro. inversion H3. contradiction.
+Qed.
+
+Lemma decidable_com : forall (c c' : com), decidable (c = c').
+Proof. 
+  intros. unfold decidable. decide equality. 
+    apply decidable_aexp. 
+    apply decidable_id.
+    apply decidable_bexp.
+    apply decidable_bexp.
+    apply decidable_aexp.
+    apply decidable_neighbor.
+    apply decidable_id.
+Qed.
+
+Lemma decidable_uid : decidable_eq uid.
+Proof. 
+  unfold decidable_eq. intros. unfold decidable. decide equality. apply dec_eq_nat.
+Qed.
+
+Lemma decidable_neighbors : decidable_eq neighbors. 
+Proof. 
+  unfold decidable_eq. intros. unfold decidable. decide equality.
+  apply decidable_uid.
+Qed. 
+
+Lemma decidable_store : decidable_eq store.
+Proof. 
+    unfold decidable_eq. unfold decidable. intros. decide equality.
+      apply dec_eq_nat.
+      apply decidable_id.
+Qed.
+
+Lemma decidable_msgs : decidable_eq (list nat).
+Proof. 
+  unfold decidable_eq. unfold decidable. intros. decide equality. 
+    apply dec_eq_nat.
+Qed. 
+
+Lemma decidable_state : decidable_eq state.
+Proof. 
+  unfold decidable_eq. unfold decidable. intros. decide equality.
+    unfold queue in *. apply decidable_msgs. apply decidable_store.
+Qed.
+
+Lemma decidable_process : decidable_eq process.
+Proof. 
+  unfold decidable_eq. intros. unfold decidable. decide equality.
+    apply decidable_neighbors.
+    apply decidable_uid.
+    apply decidable_state.
+    apply decidable_com.
+Qed.
+
+Lemma decidable_is_done_list : decidable_list_forall is_done.
+Proof.  
+  unfold decidable_list_forall. apply decidable_list_forall_if_decidable. 
+  apply decidable_process. apply decidable_is_done.
+Qed.
+
+Lemma decidable_is_sending_list : decidable_list_forall is_sending.
+Proof.  
+  unfold decidable_list_forall. apply decidable_list_forall_if_decidable. 
+  apply decidable_process. apply decidable_is_sending.
+Qed.
+
+Lemma decidable_is_receiving_list : decidable_list_forall is_receiving.
+Proof.  
+  unfold decidable_list_forall. apply decidable_list_forall_if_decidable. 
+  apply decidable_process. apply decidable_is_receiving.
+Qed.
+
