Leader.v
@@ -1,0 +1,201 @@
+Require Import Misc.
+Require Import Lang. 
+Require Import NPeano.
+
+Fixpoint allDone (ps : list process) : bool :=
+  match ps with
+    | nil => true
+    | (Process CDone _ _ _) :: ps' => allDone ps'
+    | _ => false
+  end.
+
+Definition system_halted (s : system) : Prop :=
+  match s with
+    | System ps => allDone ps = true
+  end.
+
+Inductive system_halts : system -> Prop :=
+  | SystemHalts : forall s s', 
+                    s !! s' -> 
+                    system_halted s' ->
+                    system_halts s. 
+Hint Constructors system_halts.
+
+Notation "'leader'" := (Id 0).
+Notation "'finished'" := (Id 1).
+Notation "'msg'" := (Id 2).
+Notation "'leaderA'" := (AId leader).
+Notation "'finishedA'" := (AId finished).
+Notation "'msgA'" := (AId msg).
+
+Definition leader_election : com :=
+  leader ::= (ANum 0);
+  finished ::= (ANum 0);
+  SEND AUId TO (Neighbor 0);
+  WHILEB (B= finishedA (ANum 0)) DO
+    msg <-RECEIVE;     
+    IFB (B= msgA (ANum 0))
+    THEN finished ::= (ANum 1)
+    ELSE 
+      IFB (B= msgA AUId)
+      THEN leader ::= msgA;
+           finished ::= (ANum 1);
+           SEND (ANum 0) TO (Neighbor 0)
+      ELSE 
+        IFB (B< AUId msgA)
+        THEN leader ::= msgA;
+             SEND msgA TO (Neighbor 0)
+        ELSE SEND AUId TO (Neighbor 0) 
+        FI
+      FI
+    FI
+  END.
+
+Definition leader_election_proc (n : nat) (u : uid) : process :=
+  Process leader_election empty_state (UID n) [u].
+
+Fixpoint leaderElected (n : nat) (ps : list process) : bool :=
+  match ps with 
+    | nil => true
+    | (Process _ (st,_) _ _) :: ps' => match gets leader st with 
+                                         | Some m => beq_nat n m && leaderElected n ps'
+                                         | _ => false
+                                       end
+    end.
+
+Inductive leader_elected : uid -> system -> Prop :=
+  | LeaderElected : forall n proc_list,
+                      leaderElected n proc_list = true -> 
+                      leader_elected (UID n) (System proc_list).
+Hint Constructors leader_elected. 
+
+Fixpoint maxUidN (n : nat) (ps : list process) : nat :=
+  match ps with 
+    | nil => n
+    | (Process _ _ (UID n') _) :: ps' => maxUidN (if ltb n n' then n' else n) ps'
+  end.
+
+Fixpoint max_uid (ps : list process) : option uid := 
+  match ps with 
+    | nil => None
+    | (Process _ _ (UID n) _) :: ps' => Some (UID (maxUidN n ps'))
+  end.
+
+Inductive system_leader : system -> uid -> Prop :=
+  | SystemLeader : forall proc_list u,
+                     max_uid proc_list = Some u -> 
+                     system_leader (System proc_list) u.
+Hint Constructors system_leader.
+
+Inductive correctness : system -> Prop :=
+| Correctness :  forall (n : nat) (s s' : system), 
+                   s !! s' -> 
+                   system_halted s' -> 
+                   system_leader s' (UID n) -> 
+                   leader_elected (UID n) s' -> 
+                   correctness s.
+Hint Constructors correctness.         
+
+Fixpoint n_proc_list (n : nat) : list process :=
+  match n with 
+    | 0 => []
+    | S n' => leader_election_proc n (UID (n + 1)) :: n_proc_list n'
+  end.
+
+Fixpoint range (n : nat) : list nat :=
+  match n with 
+    | 0 => []
+    | S n' => n :: range n'
+  end.
+
+Fixpoint uid_range (n : nat) : list uid :=
+  match n with 
+    | 0 => []
+    | S n' => (UID n) :: uid_range n'
+    end.       
+
+Fixpoint uid_range_two (start more : nat) : list uid :=
+  match more with 
+    | 0 => UID start :: []
+    | S more' => (UID (start + more)) :: uid_range_two start more'
+  end.
+
+Definition SnRingProcList (n : nat) := leader_election_proc (S n) (UID 1) :: n_proc_list n.
+Hint Unfold SnRingProcList.
+Definition SnProcRing (n : nat) : system := System (SnRingProcList n).
+Hint Unfold SnProcRing.
+Definition NProcRing (n : nat) : system := SnProcRing (n - 1).
+Hint Unfold NProcRing.
+
+Definition receiving (n : nat) (u : uid) (m : nat) : process := Process
+((msg <-RECEIVE;
+  IFB (B=) msgA (ANum 0) 
+  THEN finished ::= ANum 1
+  ELSE IFB (B=) msgA AUId
+    THEN leader ::= msgA; finished ::= ANum 1; SEND ANum 0 TO Neighbor 0
+    ELSE IFB (B<) AUId msgA
+      THEN leader ::= msgA; SEND msgA TO Neighbor 0
+      ELSE SEND AUId TO Neighbor 0 FI FI FI);
+           WHILEB (B=) finishedA (ANum 0)
+           DO msg <-RECEIVE;
+             IFB (B=) msgA (ANum 0) THEN finished ::= ANum 1
+             ELSE IFB (B=) msgA AUId
+               THEN leader ::= msgA;
+                    finished ::= ANum 1; SEND ANum 0 TO Neighbor 0
+               ELSE IFB (B<) AUId msgA
+                 THEN leader ::= msgA; SEND msgA TO Neighbor 0
+                 ELSE SEND AUId TO Neighbor 0 FI FI FI END)
+   (Extend (Extend Empty leader 0) finished 0, [m]) 
+   (UID n)
+   [u].
+Hint Unfold receiving.
+
+Inductive is_receiving : process -> Prop :=
+  | IsReceiving : forall p n u m, 
+                    p = receiving n u m ->
+                    is_receiving p.
+Hint Constructors is_receiving.                                   
+
+Definition modulo (m : nat) (n : nat) : nat :=
+  if ble_nat n m 
+  then n
+  else n - m.
+Hint Unfold modulo.
+
+Definition msg_in_ring_n_round_m (n : nat) (m : nat) (o : nat) : nat :=
+  if ble_nat o (S m) then n else (o - 1).
+Hint Unfold msg_in_ring_n_round_m.
+
+Definition ring_n_round_m (n : nat) (m : nat) : system :=
+  System ((receiving n (UID 1) (n - 1)) 
+            :: map (fun o => receiving o (UID (S o)) (msg_in_ring_n_round_m n m o)) (range (n - 1))).
+Hint Unfold ring_n_round_m.
+
+Lemma ring_n_round_m_correct : 
+  ring_n_round_m 5 2 = System [receiving 5 (UID 1) 4, 
+                               receiving 4 (UID 5) 3,
+                               receiving 3 (UID 4) 5,
+                               receiving 2 (UID 3) 5,
+                               receiving 1 (UID 2) 5].
+Proof.
+  unfold ring_n_round_m. simpl. 
+  unfold msg_in_ring_n_round_m. simpl.
+  reflexivity.
+Qed. 
+
+Definition initialized (n : nat) : system :=
+  ring_n_round_m n 0.
+Hint Unfold initialized.
+
+(* First, prove by induction on the list, the following lemma:
+ forall (s : system), 
+     list = proc_list system -> 
+     forall p, In p list -> is_receiving p 
+  \/ exists lr p ls, list = lr ++ p :: ls,p
+          forall p0, In p0 lr -> is_receiving p0
+       /\ ~ is_receiving p 
+       /\ exists p', p -local-> p' 
+       /\ receiving p'
+*)       
+    
+(* And then add in induction upon the list *)
