Makefile
@@ -1,0 +1,28 @@
+# Makefile for my proof
+
+all : 
+	coqc Correctness.v
+
+Correctness.vo : Correctness.v Lang.vo Leader.vo Misc.vo SfLib.vo ListExt.vo Cases.vo
+	coqc Correctness.v
+
+Cases.vo : 
+	coqc Cases.v
+
+Leader.vo : Leader.v Lang.vo Misc.vo SfLib.vo ListExt.vo
+	coqc Leader.v
+
+Misc.vo : Misc.v Lang.vo
+	coqc Misc.v
+
+Lang.vo : Lang.v SfLib.vo 
+	coqc Lang.v
+
+SfLib.vo : SfLib.v
+	coqc SfLib.v
+
+ListExt.vo : ListExt.v
+	coqc ListExt.v
+
+clean : 
+	rm -f *.vo *.v~
