README.md
@@ -1,0 +1,4 @@
+Hi, my main development is in Correctness.v
+
+It is currently unfinished, but I hope to talk to you and be able to finish it by the time I sit down for the grading meeting.
+
